messageInvariantPrototypes/twoPhaseCommit/automate_full/readme.md
@@ -1,0 +1,3 @@
+# Readme
+
+* This version does not use Application Invs
